update proof

proof/CoreLang.v
@@ -4,7 +4,7 @@ Set Warnings "-notation-overridden,-parsing".
 From PLF Require Import Maps.
 From PLF Require Import Types.
 From PLF Require Import Smallstep.
-(* From PLF Require Import Stlc. *)
+From PLF Require Import BasicConstant.
 
 Ltac invert :=
   match goal with | H : ?T |- _ =>
@@ -12,699 +12,269 @@ Ltac invert :=
                       end
   end.
 
-Module CoreLang.
-
-  (* ----------------------------------------------------------------- *)
-  (** *** Syntax *)
-
-  Inductive ty : Type :=
-  | TArrow : ty -> ty -> ty
-  | TNat   : ty
-  | TBool  : ty
-  (* | TList  : ty -> ty *)
-  (* | TTree  : ty -> ty *)
-  .
-
-  (* Inductive datatype_constant : Type := *)
-  (* | dnil *)
-  (* | dleaf *)
-  (* | dcons: datatype_constant -> datatype_constant -> datatype_constant *)
-  (* | dnode: datatype_constant -> datatype_constant -> datatype_constant. *)
-
-  (* Inductive datatype_constant : Type := *)
-  (* |  *)
-
-  Inductive constant : Type :=
-  (* | cdt: datatype_constructor -> constant -> constant -> constant *)
-  | cbool: bool -> constant
-  | cnat : nat -> constant.
-
-  Inductive biop : Type :=
-  (* | dc: datatype_constructor -> biop *)
-  | op_plus
-  | op_eq
-  | op_lt.
-
-  Inductive value : Type :=
-  | vconst : constant -> value
-  | vvar : string -> value
-  | vlam : string -> ty -> tm -> value
-  | vfix : string -> ty -> string -> ty -> tm -> value
-  | vexn
-  with tm : Type :=
-  | tvalue: value -> tm
-  | trandom
-  | tlete: string -> tm -> tm -> tm
-  | tletbiop: string -> biop -> value -> value -> tm -> tm
-  | tletapp: string -> value -> value -> tm -> tm
-  | tite: value -> tm -> tm -> tm.
-
-  Scheme value_mutual_rec := Induction for value Sort Type
-  with tm_mutual_rec := Induction for tm Sort Type.
-
-  Definition x : string := "x".
-  Definition y : string := "y".
-  Definition z : string := "z".
-
-  Global Hint Unfold x : core.
-  Global Hint Unfold y : core.
-  Global Hint Unfold z : core.
-
-  Coercion vvar : string >-> value.
-
-  Definition is_value (e: tm) :=
-    match e with
-    | tvalue _ => true
-    | _ => false
-    end.
-
-  Lemma is_value_value_exists: forall e, is_value e = true -> exists v, e = tvalue v.
-  Proof.
-    intros.
-    destruct e; inversion H; subst. exists v. auto.
-  Qed.
-
-  Fixpoint subst (x:string) (s:value) (t:tm) : tm :=
-    match t with
-    | tvalue v => tvalue (value_subst x s v)
-    | trandom => t
-    | tlete x' t1 t2 =>
-        tlete x' (subst x s t1) (if String.eqb x x' then t2 else (subst x s t2))
-    | tletbiop x' op v1 v2 t2 =>
-        tletbiop x' op (value_subst x s v1) (value_subst x s v2) (if String.eqb x x' then t2 else (subst x s t2))
-    | tletapp x' v1 v2 t2 =>
-        tletapp x' (value_subst x s v1) (value_subst x s v2) (if String.eqb x x' then t2 else (subst x s t2))
-    | tite v1 t1 t2 =>
-        tite (value_subst x s v1) (subst x s t1) (subst x s t2)
-    end
-  with value_subst (x:string) (s:value) (t:value) : value :=
-         match t with
-         |  vconst _ => t
-         |  vvar y => if String.eqb x y then s else t
-         |  vlam y T t1 => vlam y T (if String.eqb x y then t1 else (subst x s t1))
-         |  vfix f T_f y T_y t1 =>
-              vfix f T_f y T_y
-                   (if String.eqb x f then t1
-                    else if String.eqb x y then t1
-                         else (subst x s t1))
-         |  vexn => t
-         end.
-
-  Definition apply_op (op: biop) (a: nat) (b: nat): value :=
-    match op with
-    (* | dc dc =>  *)
-    | op_plus => vconst (cnat (a + b))
-    | op_eq => vconst (cbool (Nat.eqb a b))
-    | op_lt => vconst (cbool (Nat.ltb a b))
-    end.
-
-  Notation "'[' x ':=' s ']' t" := (subst x s t) (at level 20).
-  Notation "'[' x ':=' s ']v' t" := (value_subst x s t) (at level 20).
-
-  Global Hint Constructors value: core.
-  Global Hint Constructors tm: core.
-
-  Reserved Notation "t1 '-->' t2" (at level 40).
-
-  Inductive step : tm -> tm -> Prop :=
-  | ST_Random: forall n:nat, trandom --> (tvalue (vconst (cnat n)))
-  | ST_Lete1: forall x e1 e1' e, e1 --> e1' -> (tlete x e1 e) --> (tlete x e1' e)
-  | ST_Lete2: forall x v1 e, (tlete x (tvalue v1) e) --> (subst x v1 e)
-  | ST_LetOp: forall x op n1 n2 e,
-      (tletbiop x op (vconst (cnat n1)) (vconst (cnat n2)) e) --> (subst x (apply_op op n1 n2) e)
-  | ST_LetOpExn1: forall x op v1 e,
-      (tletbiop x op v1 vexn e) --> (tvalue vexn)
-  | ST_LetOpExn2: forall x op v2 e,
-      (tletbiop x op vexn v2 e) --> (tvalue vexn)
-  | ST_LetAppLam: forall T x y v_x e1 e,
-      (tletapp y ((vlam x T e1)) v_x e) --> tlete y (subst x v_x e1) e
-  | ST_LetAppFix: forall f T_f T x y v_x e1 e,
-      (tletapp y ((vfix f T_f x T e1)) v_x e) --> tlete y (subst f (vfix f T_f x T e1) (subst x v_x e1)) e
-  | ST_LetAppExn1: forall y v_x e,
-      (tletapp y vexn v_x e) --> (tvalue vexn)
-  | ST_IteTrue: forall e1 e2,
-      (tite (vconst (cbool true)) e1 e2) --> e1
-  | ST_IteFalse: forall e1 e2,
-      (tite (vconst (cbool false)) e1 e2) --> e2
-  | ST_IteExn: forall e1 e2,
-      (tite vexn e1 e2) --> (tvalue vexn)
-
-  where "t1 '-->' t2" := (step t1 t2).
-
-  Notation multistep := (multi step).
-  Notation "t1 '-->*' t2" := (multistep t1 t2) (at level 40).
-  Notation step_normal_form := (normal_form step).
-
-  Lemma value__normal : forall v, step_normal_form (tvalue v).
-  Proof with eauto.
-    intro v. unfold normal_form.
-    induction v; intro HF; inversion HF; inversion H.
-  Qed.
-
-  Global Hint Constructors step.
-
-  Definition op_ret_ty (op: biop): ty :=
-    match op with
-    | op_plus => TNat
-    | op_eq => TBool
-    | op_lt => TBool
-    end.
-
-  Definition context := partial_map ty.
-
-  Reserved Notation "Gamma '|-' t '\in' T" (at level 40).
-
-  Inductive has_type : context -> tm -> ty -> Prop :=
-  | T_Random : forall Gamma, has_type Gamma trandom TNat
-  | T_Value : forall Gamma value T,
-      value_has_type Gamma value T -> has_type Gamma (tvalue value) T
-  | T_Lete : forall Gamma x e1 e2 T1 T2,
-      has_type Gamma e1 T1 ->
-      has_type (update Gamma x T1) e2 T2 ->
-      has_type Gamma (tlete x e1 e2) T2
-  | T_LetOp : forall Gamma x op v1 v2 e2 T2,
-      value_has_type Gamma v1 TNat ->
-      value_has_type Gamma v2 TNat ->
-      has_type (update Gamma x (op_ret_ty op)) e2 T2 ->
-      has_type Gamma (tletbiop x op v1 v2 e2) T2
-  | T_LetApp : forall Gamma y v_x v_f e2 T_x T_y T2,
-      value_has_type Gamma v_x T_x ->
-      value_has_type Gamma v_f (TArrow T_x T_y) ->
-      has_type (update Gamma y T_y) e2 T2 ->
-      has_type Gamma (tletapp y v_f v_x e2) T2
-  | T_Ite: forall Gamma v e1 e2 T,
-      value_has_type Gamma v TBool ->
-      has_type Gamma e1 T ->
-      has_type Gamma e2 T ->
-      has_type Gamma (tite v e1 e2) T
-  with value_has_type : context -> value -> ty -> Prop :=
-  | T_ConstantB : forall Gamma b, value_has_type Gamma (vconst (cbool b)) TBool
-  | T_ConstantI : forall Gamma n, value_has_type Gamma (vconst (cnat n)) TNat
-  | T_Var : forall Gamma x T, Gamma x = Some T -> value_has_type Gamma (vvar x) T
-  | T_Lam : forall Gamma x T11 T12 t12,
-      has_type (update Gamma x T11) t12 T12 ->
-      value_has_type Gamma (vlam x T11 t12) (TArrow T11 T12)
-  | T_Fix : forall Gamma f x T11 T12 t12,
-      has_type (update (update Gamma f (TArrow T11 T12)) x T11) t12 T12 ->
-      value_has_type Gamma (vfix f (TArrow T11 T12) x T11 t12) (TArrow T11 T12)
-  | T_Exn : forall Gamma T, value_has_type Gamma vexn T
-
-  where "Gamma '|-' t '\in' T" := (has_type Gamma t T).
-  Notation "Gamma '|-' t '\Vin' T" := (value_has_type Gamma t T) (at level 40).
-
-  Global Hint Constructors has_type: core.
-  Global Hint Constructors value_has_type: core.
-
-  Lemma op_type_safe: forall op n1 n2, empty |- apply_op op n1 n2 \Vin op_ret_ty op.
-  Proof.
-    intro op.
-    destruct op; simpl; intros; auto.
-  Qed.
-
-  Global Hint Resolve op_type_safe: core.
-
-  Lemma nat_value_n_exists: forall v, empty |- v \Vin TNat -> (exists n, v = (vconst (cnat n))) \/ v = vexn.
-  Proof.
-    intros.
-    destruct v; inversion H; subst.
-    - left. exists n. auto.
-    - inversion H2.
-    - right. auto.
-  Qed.
-
-  Lemma bool_value_b_exists: forall v, empty |- v \Vin TBool -> (exists b, v = (vconst (cbool b))) \/ v = vexn.
-  Proof.
-    intros.
-    destruct v; inversion H; subst.
-    - left. exists b. auto.
-    - inversion H2.
-    - right. auto.
-  Qed.
-
-  Lemma arrow_value_lam_exists: forall v T1 T2,
-      empty |- v \Vin (TArrow T1 T2) ->
-              (exists f x e, v = vfix f (TArrow T1 T2) x T1 e) \/ (exists x e, v = vlam x T1 e) \/ v = vexn.
-  Proof.
-    intros.
-    destruct v; inversion H; subst.
-    - inversion H2.
-    - right. left. exists s. exists t0. auto.
-    - left. exists s, s0, t1. auto.
-    - right. auto.
-  Qed.
-
-  Lemma has_type_inv_value: forall Gamma v T, Gamma |- tvalue v \in T -> Gamma |- v \Vin T.
-  Proof.
-    intros.
-    inversion H. auto.
-  Qed.
-
-  (* ================================================================= *)
-  (** ** Properties of Typing *)
-
-  (** The proofs of progress and preservation for this enriched system
-    are essentially the same (though of course longer) as for the pure
-    STLC. *)
-
-  (* ----------------------------------------------------------------- *)
-  (** *** Progress *)
-
-  Theorem progress : forall e T,
-      empty |- e \in T -> (is_value e = true) \/ (exists e', e --> e').
-  Proof with eauto.
-    (* Theorem: Suppose empty |- t : T.  Then either
-       1. t is a value, or
-       2. t --> t' for some t'.
-     Proof: By induction on the given typing derivation. *)
-    intros t T Ht.
-    remember empty as Gamma.
-    generalize dependent HeqGamma.
-    induction Ht; intros HeqGamma; subst; simpl.
-    - right. exists (tvalue (vconst (cnat 0)))...
-    - left...
-    - right. destruct IHHt1; auto.
-      destruct (is_value_value_exists _ H) as (v' & Hv'). subst. exists ([ x0 := v' ] e2)...
-      destruct H as (e1' & He'). exists (tlete x0 e1' e2)...
-    - right.
-      apply nat_value_n_exists in H0.
-      apply nat_value_n_exists in H.
-      destruct H0, H.
-      + destruct H0 as (n2 & H2). destruct H as (n1 & H1). subst. exists ([x0 := (apply_op op n1 n2)] e2)...
-      + exists (tvalue vexn). subst...
-      + exists (tvalue vexn). subst...
-      + exists (tvalue vexn). subst...
-   - right.
-     destruct (arrow_value_lam_exists _ _ _ H0).
-     + destruct H1 as (f & x & e1 & H1). subst. exists (tlete y0 ([f:= (vfix f (TArrow T_x T_y) x T_x e1)] [x:= v_x] e1) e2)...
-     + destruct H1.
-       destruct H1 as (x & e1 & H1). subst. exists (tlete y0 ([x:= v_x] e1) e2)...
-       subst. eauto...
-   - right.
-      destruct (bool_value_b_exists _ H).
-     + destruct H0 as (b & Hb); destruct b; subst...
-     + exists (tvalue vexn). subst...
-  Qed.
-
-  Definition halts (t:tm) : Prop :=  exists t', t -->* t' /\ is_value t' = true.
-
-  Lemma value_halts : forall v, halts (tvalue v).
-  Proof.
-    intros v. unfold halts. exists (tvalue v). split; auto.
-  Qed.
-
-  (* logical relation *)
-  Fixpoint R (T:ty) (t:tm) : Prop :=
-    empty |- t \in T /\ halts t /\
-                    (match T with
-                     | TBool => True
-                     | TNat => True
-                     | TArrow T1 T2 => forall f y v,
-                         R T1 (tvalue v) ->
-                         R T2 (tlete f t (tletapp y (vvar f) v
-                                                  (tvalue (vvar y))))
-                     end).
-
-  Lemma R_halts : forall {T} {t}, R T t -> halts t.
-  Proof.
-    intros.
-    destruct T; unfold R in H; destruct H as [_ [H _]]; assumption.
-  Qed.
-
-  Lemma R_typable_empty : forall {T} {t}, R T t -> empty |- t \in T.
-  Proof.
-    intros.
-    destruct T; unfold R in H; destruct H as [H _]; assumption.
-  Qed.
-
-
-  Lemma weakening1:  forall c T Gamma Gamma', includedin Gamma Gamma' -> Gamma |- vconst c \Vin T -> Gamma' |- vconst c \Vin T.
-  Proof.
-    intros.
-    inversion H0; subst; auto.
-  Qed.
-
-  Lemma weakening2: (forall (s : string) (T : ty) (Gamma Gamma' : partial_map ty),
-        includedin Gamma Gamma' -> Gamma |- s \Vin T -> Gamma' |- s \Vin T).
-  Proof.
-    intros.
-    inversion H0; subst; auto.
-  Qed.
-
-  Lemma weakening3: (forall (s : string) (t : ty) (t0 : tm),
-        (forall (T : ty) (Gamma Gamma' : partial_map ty),
-         includedin Gamma Gamma' -> Gamma |- t0 \in T -> Gamma' |- t0 \in T) ->
-        forall (T : ty) (Gamma Gamma' : partial_map ty),
-        includedin Gamma Gamma' -> Gamma |- vlam s t t0 \Vin T -> Gamma' |- vlam s t t0 \Vin T).
-  Proof.
-    intros.
-    inversion H1; subst; eauto 7 using includedin_update.
-  Qed.
-
-  Lemma weakening4:
-    forall (s : string) (t : ty) (s0 : string) (t0 : ty) (t1 : tm),
-      (forall (T : ty) (Gamma Gamma' : partial_map ty), includedin Gamma Gamma' -> Gamma |- t1 \in T -> Gamma' |- t1 \in T) ->
-      forall (T : ty) (Gamma Gamma' : partial_map ty),
-        includedin Gamma Gamma' -> Gamma |- vfix s t s0 t0 t1 \Vin T -> Gamma' |- vfix s t s0 t0 t1 \Vin T.
-  Proof.
-    intros.
-    inversion H1; subst; eauto 7 using includedin_update.
-  Qed.
-
-
-  Lemma weakening5: (forall (T : ty) (Gamma Gamma' : partial_map ty),
-                        includedin Gamma Gamma' -> Gamma |- vexn \Vin T -> Gamma' |- vexn \Vin T).
-  Proof.
-    intros.
-    inversion H0; subst; eauto 7 using includedin_update.
-  Qed.
-
-  Lemma weakening6:
-    (forall v : value,
-        (forall (T : ty) (Gamma Gamma' : partial_map ty), includedin Gamma Gamma' -> Gamma |- v \Vin T -> Gamma' |- v \Vin T) ->
-        forall (T : ty) (Gamma Gamma' : partial_map ty),
-          includedin Gamma Gamma' -> Gamma |- tvalue v \in T -> Gamma' |- tvalue v \in T).
-  Proof.
-    intros.
-    inversion H1; subst; eauto 7 using includedin_update.
-  Qed.
-
-  Lemma weakening7:
-    (forall (T : ty) (Gamma Gamma' : partial_map ty),
-        includedin Gamma Gamma' -> Gamma |- trandom \in T -> Gamma' |- trandom \in T).
-  Proof.
-    intros.
-    inversion H0; subst; eauto 7 using includedin_update.
-  Qed.
-
-  Lemma weakening8:
-    (forall (s : string) (t : tm),
-        (forall (T : ty) (Gamma Gamma' : partial_map ty), includedin Gamma Gamma' -> Gamma |- t \in T -> Gamma' |- t \in T) ->
-        forall t0 : tm,
-          (forall (T : ty) (Gamma Gamma' : partial_map ty),
-              includedin Gamma Gamma' -> Gamma |- t0 \in T -> Gamma' |- t0 \in T) ->
-          forall (T : ty) (Gamma Gamma' : partial_map ty),
-            includedin Gamma Gamma' -> Gamma |- tlete s t t0 \in T -> Gamma' |- tlete s t t0 \in T).
-  Proof.
-    intros.
-    inversion H2; subst; eauto 7 using includedin_update.
-  Qed.
-
-  Lemma weakening9:
-    (forall (s : string) (b : biop) (v : value),
-        (forall (T : ty) (Gamma Gamma' : partial_map ty),
-            includedin Gamma Gamma' -> Gamma |- v \Vin T -> Gamma' |- v \Vin T) ->
-        forall v0 : value,
-          (forall (T : ty) (Gamma Gamma' : partial_map ty),
-              includedin Gamma Gamma' -> Gamma |- v0 \Vin T -> Gamma' |- v0 \Vin T) ->
-          forall t : tm,
-            (forall (T : ty) (Gamma Gamma' : partial_map ty), includedin Gamma Gamma' -> Gamma |- t \in T -> Gamma' |- t \in T) ->
-            forall (T : ty) (Gamma Gamma' : partial_map ty),
-              includedin Gamma Gamma' -> Gamma |- tletbiop s b v v0 t \in T -> Gamma' |- tletbiop s b v v0 t \in T).
-  Proof.
-    intros.
-    inversion H3; subst; eauto 7 using includedin_update.
-  Qed.
-
-  Lemma weakening10:
-    (forall (s : string) (v : value),
-        (forall (T : ty) (Gamma Gamma' : partial_map ty),
-            includedin Gamma Gamma' -> Gamma |- v \Vin T -> Gamma' |- v \Vin T) ->
-        forall v0 : value,
-          (forall (T : ty) (Gamma Gamma' : partial_map ty),
-              includedin Gamma Gamma' -> Gamma |- v0 \Vin T -> Gamma' |- v0 \Vin T) ->
-          forall t : tm,
-            (forall (T : ty) (Gamma Gamma' : partial_map ty), includedin Gamma Gamma' -> Gamma |- t \in T -> Gamma' |- t \in T) ->
-            forall (T : ty) (Gamma Gamma' : partial_map ty),
-              includedin Gamma Gamma' -> Gamma |- tletapp s v v0 t \in T -> Gamma' |- tletapp s v v0 t \in T).
-  Proof.
-    intros.
-    inversion H3; subst; eauto 7 using includedin_update.
-  Qed.
-
-  Lemma weakening11:
-        (forall v : value,
-            (forall (T : ty) (Gamma Gamma' : partial_map ty),
-                includedin Gamma Gamma' -> Gamma |- v \Vin T -> Gamma' |- v \Vin T) ->
-            forall t : tm,
-              (forall (T : ty) (Gamma Gamma' : partial_map ty), includedin Gamma Gamma' -> Gamma |- t \in T -> Gamma' |- t \in T) ->
-              forall t0 : tm,
-                (forall (T : ty) (Gamma Gamma' : partial_map ty),
-                    includedin Gamma Gamma' -> Gamma |- t0 \in T -> Gamma' |- t0 \in T) ->
-                forall (T : ty) (Gamma Gamma' : partial_map ty),
-                  includedin Gamma Gamma' -> Gamma |- tite v t t0 \in T -> Gamma' |- tite v t t0 \in T).
-  Proof.
-    intros.
-    inversion H3; subst; eauto 7 using includedin_update.
-  Qed.
-
-  Lemma weakening : forall e T Gamma Gamma',
-      includedin Gamma Gamma' ->
-      (Gamma  |- e \in T -> Gamma' |- e \in T).
-  Proof.
-    intro e.
-    apply
-      (tm_mutual_rec
-         (fun v => forall T Gamma Gamma', includedin Gamma Gamma' -> (Gamma  |- v \Vin T -> Gamma' |- v \Vin T))
-         (fun e => forall T Gamma Gamma', includedin Gamma Gamma' -> (Gamma  |- e \in T -> Gamma' |- e \in T))
-         weakening1 weakening2 weakening3
-         weakening4 weakening5 weakening6 weakening7 weakening8 weakening9 weakening10 weakening11
-      ).
-  Qed.
-
-  Lemma value_weakening : forall e T Gamma Gamma',
-      includedin Gamma Gamma' ->
-      (Gamma  |- e \Vin T -> Gamma' |- e \Vin T).
-  Proof.
-    intros.
-    apply weakening with (e:=tvalue e) (T:=T) in H; auto.
-    inversion H; subst; auto.
-  Qed.
-
-  Lemma weakening_empty : forall Gamma t T,
-      empty |- t \in T  -> Gamma |- t \in T.
-  Proof.
-    intros Gamma t T.
-    eapply weakening.
-    discriminate.
-  Qed.
-
-  Lemma value_weakening_empty : forall Gamma t T,
-      empty |- t \Vin T  -> Gamma |- t \Vin T.
-  Proof.
-    intros Gamma t T H.
-    assert (empty |- (tvalue t) \in T). auto.
-    apply weakening_empty with (Gamma:=Gamma) in H0. inversion H0; subst; auto.
-  Qed.
-
-  Lemma substitution_preserves_typing1:
-  (forall (c : constant) (Gamma : partial_map ty) (x : string) (U : ty) (v : value) (T : ty),
-        (x |-> U; Gamma) |- vconst c \Vin T -> empty |- v \Vin U -> Gamma |- [x := v ]v vconst c \Vin T).
-  Proof.
-    intros. inversion H; clear H; subst; simpl; eauto.
-  Qed.
-
-  Lemma substitution_preserves_typing2:
-    (forall (s : string) (Gamma : partial_map ty) (x : string) (U : ty) (v : value) (T : ty),
-        (x |-> U; Gamma) |- s \Vin T -> empty |- v \Vin U -> Gamma |- [x := v ]v s \Vin T).
-  Proof.
-    intros. inversion H; clear H; subst; simpl; eauto.
-    rename s into y. rename x0 into x.
-    destruct (eqb_spec x y); subst.
-      + (* x=y *)
-        rewrite update_eq in H3.
-        injection H3 as H3; subst.
-        apply value_weakening_empty. assumption.
-      + (* x<>y *)
-        apply T_Var. rewrite update_neq in H3; auto.
-  Qed.
-
-  Lemma substitution_preserves_typing3:
-  (forall (s : string) (t : ty) (t0 : tm),
-        (forall (Gamma : partial_map ty) (x : string) (U : ty) (v : value) (T : ty),
-         (x |-> U; Gamma) |- t0 \in T -> empty |- v \Vin U -> Gamma |- [x := v] t0 \in T) ->
-        forall (Gamma : partial_map ty) (x : string) (U : ty) (v : value) (T : ty),
-        (x |-> U; Gamma) |- vlam s t t0 \Vin T -> empty |- v \Vin U -> Gamma |- [x := v ]v vlam s t t0 \Vin T).
-  Proof.
-    intros. inversion H0; clear H0; subst; simpl; eauto.
-    rename s into y. rename x0 into x.
-    destruct (eqb_spec x y); subst; apply T_Lam.
-    + (* x=y *)
-      rewrite update_shadow in H7. assumption.
-    + (* x<>y *)
-      apply H with (U:=U); auto.
-      rewrite update_permute; auto.
-  Qed.
-
-  Lemma substitution_preserves_typing_fix:
-    forall (s : string) (t0 : ty) (s0 : string) (t1 : ty) (t2 : tm),
-      (forall (Gamma : partial_map ty) (x : string) (U : ty) (v : value) (T : ty),
-          (x |-> U; Gamma) |- t2 \in T -> empty |- v \Vin U -> Gamma |- [x := v] t2 \in T) ->
-      forall (Gamma : partial_map ty) (x0 : string) (U : ty) (v : value) (T : ty),
-        (x0 |-> U; Gamma) |- vfix s t0 s0 t1 t2 \Vin T -> empty |- v \Vin U -> Gamma |- [x0 := v ]v vfix s t0 s0 t1 t2 \Vin T.
-  Proof.
-    intros. inversion H0; clear H0; subst; simpl; eauto.
-    rename s into y. rename x0 into x.
-    destruct (eqb_spec x y); subst; apply T_Fix.
-    + (* x=y *)
-      rewrite update_shadow in H9. assumption.
-    + (* x<>y *)
-      destruct (eqb_spec x s0); subst.
-      - rewrite update_permute in H9; auto.
-        rewrite update_shadow in H9; auto.
-        rewrite update_permute in H9; auto.
-      - apply H with (U:=U); auto.
-        rewrite update_permute; auto.
-        rewrite (update_permute _ _ x y); auto.
-  Qed.
-
-  Lemma substitution_preserves_typing4:
-    (forall (Gamma : partial_map ty) (x : string) (U : ty) (v : value) (T : ty),
-        (x |-> U; Gamma) |- vexn \Vin T -> empty |- v \Vin U -> Gamma |- [x := v ]v vexn \Vin T).
-  Proof.
-    intros. inversion H0; clear H0; subst; simpl; eauto.
-    Qed.
-
-  Lemma substitution_preserves_typing5:
-    (forall v : value,
-        (forall (Gamma : partial_map ty) (x : string) (U : ty) (v0 : value) (T : ty),
-            (x |-> U; Gamma) |- v \Vin T -> empty |- v0 \Vin U -> Gamma |- [x := v0 ]v v \Vin T) ->
-        forall (Gamma : partial_map ty) (x : string) (U : ty) (v0 : value) (T : ty),
-          (x |-> U; Gamma) |- tvalue v \in T -> empty |- v0 \Vin U -> Gamma |- [x := v0] tvalue v \in T).
-  Proof.
-    intros. inversion H0; clear H0; subst; simpl; eauto.
-  Qed.
-
-  Lemma substitution_preserves_typing6:
-    (forall (Gamma : partial_map ty) (x : string) (U : ty) (v : value) (T : ty),
-        (x |-> U; Gamma) |- trandom \in T -> empty |- v \Vin U -> Gamma |- [x := v] trandom \in T).
-  Proof.
-    intros. inversion H; clear H; subst; simpl; eauto.
-  Qed.
-
-  Lemma substitution_preserves_typing7:
-    (forall (s : string) (t : tm),
-        (forall (Gamma : partial_map ty) (x : string) (U : ty) (v : value) (T : ty),
-            (x |-> U; Gamma) |- t \in T -> empty |- v \Vin U -> Gamma |- [x := v] t \in T) ->
-        forall t0 : tm,
-          (forall (Gamma : partial_map ty) (x : string) (U : ty) (v : value) (T : ty),
-              (x |-> U; Gamma) |- t0 \in T -> empty |- v \Vin U -> Gamma |- [x := v] t0 \in T) ->
-          forall (Gamma : partial_map ty) (x : string) (U : ty) (v : value) (T : ty),
-            (x |-> U; Gamma) |- tlete s t t0 \in T -> empty |- v \Vin U -> Gamma |- [x := v] tlete s t t0 \in T).
-    Proof.
-      intros. inversion H1; clear H1; subst; simpl; eauto.
-      rename s into y. rename x0 into x.
-      destruct (eqb_spec x y); subst.
-      + (* x=y *)
-        rewrite update_shadow in H9.
-        apply T_Lete with (T1:= T1); auto. apply H with (U:=U); auto.
-      + (* x<>y *)
-        apply T_Lete with (T1:= T1); auto. apply H with (U:=U); auto.
-        rewrite update_permute in H9; auto. apply H0 with (U:=U); auto.
-    Qed.
-
-  Lemma substitution_preserves_typing8:
-    (forall (s : string) (b : biop) (v : value),
-        (forall (Gamma : partial_map ty) (x : string) (U : ty) (v0 : value) (T : ty),
-            (x |-> U; Gamma) |- v \Vin T -> empty |- v0 \Vin U -> Gamma |- [x := v0 ]v v \Vin T) ->
-        forall v0 : value,
-          (forall (Gamma : partial_map ty) (x : string) (U : ty) (v1 : value) (T : ty),
-              (x |-> U; Gamma) |- v0 \Vin T -> empty |- v1 \Vin U -> Gamma |- [x := v1 ]v v0 \Vin T) ->
-          forall t : tm,
-            (forall (Gamma : partial_map ty) (x : string) (U : ty) (v1 : value) (T : ty),
-                (x |-> U; Gamma) |- t \in T -> empty |- v1 \Vin U -> Gamma |- [x := v1] t \in T) ->
-            forall (Gamma : partial_map ty) (x : string) (U : ty) (v1 : value) (T : ty),
-              (x |-> U; Gamma) |- tletbiop s b v v0 t \in T ->  empty |- v1 \Vin U -> Gamma |- [x := v1] tletbiop s b v v0 t \in T).
-    Proof.
-      intros. inversion H2; clear H2; subst; simpl; eauto.
-      rename s into y. rename x0 into x.
-      destruct (eqb_spec x y); subst.
-      + (* x=y *)
-        rewrite update_shadow in H13.
-        apply T_LetOp; auto. apply H with (U:=U); auto. apply H0 with (U:=U); auto.
-      + (* x<>y *)
-        apply T_LetOp; auto. apply H with (U:=U); auto.
-        rewrite update_permute in H13; auto. apply H0 with (U:=U); auto.
-        rewrite update_permute in H13; auto. apply H1 with (U:=U); auto.
-    Qed.
-
-  Lemma substitution_preserves_typing9:
-    (forall (s : string) (v : value),
-        (forall (Gamma : partial_map ty) (x : string) (U : ty) (v0 : value) (T : ty),
-            (x |-> U; Gamma) |- v \Vin T -> empty |- v0 \Vin U -> Gamma |- [x := v0 ]v v \Vin T) ->
-        forall v0 : value,
-          (forall (Gamma : partial_map ty) (x : string) (U : ty) (v1 : value) (T : ty),
-              (x |-> U; Gamma) |- v0 \Vin T -> empty |- v1 \Vin U -> Gamma |- [x := v1 ]v v0 \Vin T) ->
-          forall t : tm,
-            (forall (Gamma : partial_map ty) (x : string) (U : ty) (v1 : value) (T : ty),
-                (x |-> U; Gamma) |- t \in T -> empty |- v1 \Vin U -> Gamma |- [x := v1] t \in T) ->
-            forall (Gamma : partial_map ty) (x : string) (U : ty) (v1 : value) (T : ty),
-              (x |-> U; Gamma) |- tletapp s v v0 t \in T -> empty |- v1 \Vin U -> Gamma |- [x := v1] tletapp s v v0 t \in T).
-   Proof.
-      intros. inversion H2; clear H2; subst; simpl; eauto.
-      rename s into y. rename x0 into x.
-      destruct (eqb_spec x y); subst.
-      + (* x=y *)
-        rewrite update_shadow in H12.
-        apply T_LetApp with (T_x:=T_x) (T_y:=T_y); auto. apply H0 with (U:=U); auto. apply H with (U:=U); auto.
-      + (* x<>y *)
-        rewrite update_permute in H12; auto.
-        apply T_LetApp with (T_x:=T_x) (T_y:=T_y); auto.
-        apply H0 with (U:=U); auto.
-        apply H with (U:=U); auto.
-        apply H1 with (U:=U); auto.
-   Qed.
-
-  Lemma substitution_preserves_typing10:
-    (forall v : value,
-        (forall (Gamma : partial_map ty) (x : string) (U : ty) (v0 : value) (T : ty),
-            (x |-> U; Gamma) |- v \Vin T -> empty |- v0 \Vin U -> Gamma |- [x := v0 ]v v \Vin T) ->
-        forall t : tm,
-          (forall (Gamma : partial_map ty) (x : string) (U : ty) (v0 : value) (T : ty),
-              (x |-> U; Gamma) |- t \in T -> empty |- v0 \Vin U -> Gamma |- [x := v0] t \in T) ->
-          forall t0 : tm,
-            (forall (Gamma : partial_map ty) (x : string) (U : ty) (v0 : value) (T : ty),
-                (x |-> U; Gamma) |- t0 \in T -> empty |- v0 \Vin U -> Gamma |- [x := v0] t0 \in T) ->
-            forall (Gamma : partial_map ty) (x : string) (U : ty) (v0 : value) (T : ty),
-              (x |-> U; Gamma) |- tite v t t0 \in T -> empty |- v0 \Vin U -> Gamma |- [x := v0] tite v t t0 \in T).
-  Proof.
-    intros. inversion H2; clear H2; subst; simpl; eauto.
-  Qed.
-
-
-  Lemma substitution_preserves_typing : forall t Gamma x U v T,
-      (x |-> U ; Gamma) |- t \in T ->  empty |- v \Vin U  ->  Gamma |- [x:=v]t \in T.
-  Proof with eauto.
-    intro t.
-    apply (tm_mutual_rec
-             (fun ev => forall Gamma x U v T, (x |-> U ; Gamma) |- ev \Vin T ->  empty |- v \Vin U ->  Gamma |- [x:=v]v ev \Vin T)
-             (fun e => forall Gamma x U v T, (x |-> U ; Gamma) |- e \in T ->  empty |- v \Vin U ->  Gamma |- [x:=v] e \in T)
-             substitution_preserves_typing1 substitution_preserves_typing2 substitution_preserves_typing3
-             substitution_preserves_typing_fix
-             substitution_preserves_typing4 substitution_preserves_typing5 substitution_preserves_typing6
-             substitution_preserves_typing7 substitution_preserves_typing8 substitution_preserves_typing9
-             substitution_preserves_typing10
-          ).
-  Qed.
-
-  Theorem preservation : forall t t' T,
-      empty |- t \in T  ->
-                    t --> t'  ->
-                    empty |- t' \in T.
-  Proof with eauto.
-    intros t t' T HT. generalize dependent t'.
-    remember empty as Gamma.
-    induction HT;
-      intros t' HE; subst; inversion HE; subst...
-    - apply substitution_preserves_typing with T1...
-      inversion HT1; subst...
-    - apply substitution_preserves_typing with (op_ret_ty op)...
-    - apply T_Lete with (T1 := T_y)...
-      apply substitution_preserves_typing with T_x...
-      inversion H0; subst...
-    - apply T_Lete with (T1 := T_y)...
-      apply substitution_preserves_typing with (TArrow T_x T_y)...
-      apply substitution_preserves_typing with T_x...
-      inversion H0; subst...
-  Qed.
-
-End CoreLang.
+
+(* ----------------------------------------------------------------- *)
+(** *** Syntax *)
+
+Inductive basic_ty : Type :=
+| TNat   : basic_ty
+| TBool  : basic_ty
+| TList  : basic_ty -> basic_ty
+| TTree  : basic_ty -> basic_ty.
+
+Inductive constant : Type :=
+| cnil: basic_ty -> constant
+| cleaf: basic_ty -> constant
+| ccons: basic_ty -> constant -> constant -> constant
+| cnode: basic_ty -> constant -> constant -> constant -> constant
+| cbool: bool -> constant
+| cnat : nat -> constant.
+
+Inductive ty : Type :=
+| TBasic : basic_ty -> ty
+| TArrow : ty -> ty -> ty.
+
+Definition state := total_map constant.
+(* The second constant is the self reference *)
+Definition refinement : Type := state -> constant -> Prop.
+Implicit Type HH : refinement.
+
+Definition closed_r (P:constant -> Prop) : refinement := fun _ => P.
+
+Inductive oty : Type :=
+| BaseOver: basic_ty -> refinement -> oty.
+
+Inductive uty : Type :=
+| BaseUnder: basic_ty -> refinement -> uty
+| DependArrow : string -> oty -> uty -> uty
+| IndependArrow : uty -> uty -> uty.
+
+Inductive outy : Type :=
+| Uty: uty -> outy
+| Oty: oty -> outy.
+
+Coercion Uty : uty >-> outy.
+Coercion Oty : oty >-> outy.
+Coercion TBasic : basic_ty >-> ty.
+Coercion cbool : bool >-> constant.
+Coercion cnat : nat >-> constant.
+
+Definition ot_to_ut (ot: oty) :=
+  match ot with
+  | BaseOver t phi => BaseUnder t phi
+  end.
+
+Notation " t1 't-->' t2 " := (TArrow t1 t2) (at level 20).
+Notation "'[[v:' t '|' r ']]'" := (BaseUnder t r) (at level 20).
+Notation "'{{v:' t '|' r '}}'" := (BaseOver t r) (at level 20).
+Notation " x 'o:' oty 'o-->' retty " := (DependArrow x oty retty) (at level 20).
+Notation " uty 'u-->' retty " := (IndependArrow uty retty) (at level 20).
+
+Fixpoint erase (uty: uty) : ty :=
+  match uty with
+  | [[v: T | _ ]] => T
+  | _ o: {{v: T1 | _ }} o--> retty => T1 t--> (erase retty)
+  | t1 u--> t2 => (erase t1) t--> (erase t2)
+  end.
+
+Definition oty_erase (aty: oty): ty :=
+  match aty with
+  | ({{v: T | _ }}) => T
+  end.
+
+Definition outy_erase (aty: outy): ty :=
+  match aty with
+  | Uty ty => erase ty
+  | Oty ty => oty_erase ty
+  end.
+
+Inductive biop : Type :=
+| op_plus
+| op_eq
+| op_lt.
+
+Inductive value : Type :=
+| vconst : constant -> value
+| vvar : string -> value
+| vlam : string -> outy -> tm -> value
+| vfix : string -> uty -> string -> oty -> tm -> value
+| vexn
+with tm : Type :=
+| tvalue: value -> tm
+| trandom
+| tlete: string -> tm -> tm -> tm
+| tletbiop: string -> biop -> value -> value -> tm -> tm
+| tlets: string -> value -> tm -> tm
+| tletcons: string -> basic_ty -> value -> value -> tm -> tm
+| tletnode: string -> basic_ty -> value -> value -> value -> tm -> tm
+| tletapp: string -> value -> value -> tm -> tm
+| tmatchb: value -> tm -> tm -> tm
+| tmatchn: value -> tm -> string -> tm -> tm
+| tmatchl: basic_ty -> value -> tm -> string -> string -> tm -> tm
+| tmatcht: basic_ty -> value -> tm -> string -> string -> string -> tm -> tm.
+
+Scheme value_mutual_rec := Induction for value Sort Type
+    with tm_mutual_rec := Induction for tm Sort Type.
+
+Coercion vvar : string >-> value.
+
+Definition is_value (e: tm) :=
+  match e with
+  | tvalue _ => true
+  | _ => false
+  end.
+
+Lemma is_value_value_exists: forall e, is_value e = true -> exists v, e = tvalue v.
+Proof.
+  intros.
+  destruct e; inversion H; subst. exists v. auto.
+Qed.
+
+Fixpoint subst (x:string) (s:value) (t:tm) : tm :=
+  match t with
+  | tvalue v => tvalue (value_subst x s v)
+  | trandom => t
+  | tlete x' t1 t2 =>
+      tlete x' (subst x s t1) (if String.eqb x x' then t2 else (subst x s t2))
+  | tletbiop x' op v1 v2 t2 =>
+      tletbiop x' op (value_subst x s v1) (value_subst x s v2) (if String.eqb x x' then t2 else (subst x s t2))
+  | tlets x' v1 t2 =>
+      tlets x' (value_subst x s v1)
+            (if String.eqb x x' then t2 else (subst x s t2))
+  | tletcons x' T v1 v2 t2 =>
+      tletcons x' T (value_subst x s v1) (value_subst x s v2)
+               (if String.eqb x x' then t2 else (subst x s t2))
+  | tletnode x' T v1 v2 v3 t2 =>
+      tletnode x' T (value_subst x s v1) (value_subst x s v2) (value_subst x s v3) (if String.eqb x x' then t2 else (subst x s t2))
+  | tletapp x' v1 v2 t2 =>
+      tletapp x' (value_subst x s v1) (value_subst x s v2)
+              (if String.eqb x x' then t2 else (subst x s t2))
+  | tmatchb v1 t1 t2 =>
+      tmatchb (value_subst x s v1) (subst x s t1) (subst x s t2)
+  | tmatchn v1 t1 n' t2 =>
+      tmatchn (value_subst x s v1) (subst x s t1) n'
+              (if String.eqb x n' then t2 else (subst x s t2))
+  | tmatchl T v e1 h t e2 =>
+      tmatchl T (value_subst x s v)
+              (subst x s e1)
+              h t
+              (if String.eqb x h then e2
+               else if String.eqb x t then e2
+                    else (subst x s e2))
+  | tmatcht T v e1 root lt rt e2 =>
+      tmatcht T (value_subst x s v)
+              (subst x s e1)
+              root lt rt
+              (if String.eqb x root then e2
+               else if String.eqb x lt then e2
+                    else if String.eqb x rt then e2
+                         else (subst x s e2))
+  end
+with value_subst (x:string) (s:value) (t:value) : value :=
+       match t with
+       |  vconst _ => t
+       |  vvar y => if String.eqb x y then s else t
+       |  vlam y T t1 => vlam y T (if String.eqb x y then t1 else (subst x s t1))
+       |  vfix f T_f y T_y t1 =>
+            vfix f T_f y T_y
+                 (if String.eqb x f then t1
+                  else if String.eqb x y then t1
+                       else (subst x s t1))
+       |  vexn => t
+       end.
+
+Definition apply_op (op: biop) (a: nat) (b: nat): constant :=
+  match op with
+  | op_plus =>  (cnat (a + b))
+  | op_eq =>  (cbool (Nat.eqb a b))
+  | op_lt =>  (cbool (Nat.ltb a b))
+  end.
+
+Notation "'[' x ':=' s ']' t" := (subst x s t) (at level 20).
+Notation "'[' x ':=' s ']v' t" := (value_subst x s t) (at level 20).
+
+Global Hint Constructors value: core.
+Global Hint Constructors tm: core.
+
+Reserved Notation "t1 '-->' t2" (at level 40).
+
+Inductive step : tm -> tm -> Prop :=
+| ST_Random: forall n:nat, trandom --> (tvalue (vconst (cnat n)))
+| ST_Lete1: forall x e1 e1' e, e1 --> e1' -> (tlete x e1 e) --> (tlete x e1' e)
+| ST_Lete2: forall x v1 e, (tlete x (tvalue v1) e) --> (subst x v1 e)
+| ST_LetOp: forall x op n1 n2 e,
+    (tletbiop x op (vconst (cnat n1)) (vconst (cnat n2)) e) --> (subst x (vconst (apply_op op n1 n2)) e)
+| ST_LetOpExn1: forall x op v1 e,
+    (tletbiop x op v1 vexn e) --> (tvalue vexn)
+| ST_LetOpExn2: forall x op v2 e,
+    (tletbiop x op vexn v2 e) --> (tvalue vexn)
+| ST_LetS: forall x n e,
+    (tlets x (vconst (cnat n)) e) --> (subst x (vconst (cnat (n + 1))) e)
+| ST_LetSExn: forall x e,
+    (tlets x vexn e) --> (tvalue vexn)
+| ST_LetCons: forall x T c1 c2 e,
+    (tletcons x T (vconst c1) (vconst c2) e) --> (subst x (vconst (ccons T c1 c2)) e)
+| ST_LetConsExn1: forall x T v1 e,
+    (tletcons x T v1 vexn e) --> (tvalue vexn)
+| ST_LetConsExn2: forall x T v2 e,
+    (tletcons x T vexn v2 e) --> (tvalue vexn)
+| ST_LetNode: forall x T c1 c2 c3 e,
+    (tletnode x T (vconst c1) (vconst c2) (vconst c3) e) --> (subst x (vconst (cnode T c1 c2 c3)) e)
+| ST_LetNodeExn1: forall x T v1 v2 e,
+    (tletnode x T v1 v2 vexn e) --> (tvalue vexn)
+| ST_LetNodeExn2: forall x T v1 v3 e,
+    (tletnode x T v1 vexn v3 e) --> (tvalue vexn)
+| ST_LetNodeExn3: forall x T v2 v3 e,
+    (tletnode x T vexn v2 v3 e) --> (tvalue vexn)
+| ST_LetAppLam: forall T x y v_x e1 e,
+    (tletapp y ((vlam x T e1)) v_x e) --> tlete y (subst x v_x e1) e
+| ST_LetAppFix: forall f T_f T x y v_x e1 e,
+    (tletapp y ((vfix f T_f x T e1)) v_x e) --> tlete y (subst f (vfix f T_f x T e1) (subst x v_x e1)) e
+| ST_LetAppExn1: forall y v_x e,
+    (tletapp y vexn v_x e) --> (tvalue vexn)
+| ST_Matchbtrue: forall e1 e2,
+    (tmatchb (vconst (cbool true)) e1 e2) --> e1
+| ST_Matchbfalse: forall e1 e2,
+    (tmatchb (vconst (cbool false)) e1 e2) --> e2
+| ST_MatchbExn: forall e1 e2,
+    (tmatchb vexn e1 e2) --> (tvalue vexn)
+| ST_Matchno: forall e1 y e2,
+    (tmatchn (vconst (cnat 0)) e1 y e2) --> e1
+| ST_Matchns: forall n e1 y e2,
+    (tmatchn (vconst (cnat (1 + n))) e1 y e2) --> (subst y (vconst (cnat n)) e2)
+| ST_MatchnExn: forall e1 y e2,
+    (tmatchn vexn e1 y e2) --> (tvalue vexn)
+| ST_Matchlnil: forall T e1 h t e2,
+    (tmatchl T (vconst (cnil T)) e1 h t e2) --> e1
+| ST_Matchlcons: forall T ch ct e1 h t e2,
+    (tmatchl T (vconst (ccons T ch ct)) e1 h t e2) --> (subst t (vconst ct) (subst h (vconst ch) e2))
+| ST_MatchlExn: forall T e1 h t e2,
+    (tmatchl T vexn e1 h t e2) --> (tvalue vexn)
+| ST_Matchtleaf: forall T e1 root lt rt e2,
+    (tmatcht T (vconst (cleaf T)) e1 root lt rt e2) --> e1
+| ST_Matchtnode: forall T croot clt crt e1 root lt rt e2,
+    (tmatcht T (vconst (cnode T croot clt crt)) e1 root lt rt e2) --> (subst rt (vconst crt) (subst lt (vconst clt) (subst root (vconst croot) e2)))
+| ST_MatchExn: forall T e1 root lt rt e2,
+    (tmatcht T vexn e1 root lt rt e2) --> (tvalue vexn)
+
+where "t1 '-->' t2" := (step t1 t2).
+
+Notation multistep := (multi step).
+Notation "t1 '-->*' t2" := (multistep t1 t2) (at level 40).
+Notation step_normal_form := (normal_form step).
+
+Lemma value__normal : forall v, step_normal_form (tvalue v).
+Proof with eauto.
+  intro v. unfold normal_form.
+  induction v; intro HF; inversion HF; inversion H.
+Qed.
+
+Global Hint Constructors step: core.
+
+Definition op_ret_ty (op: biop): basic_ty :=
+  match op with
+  | op_plus => TNat
+  | op_eq => TBool
+  | op_lt => TBool
+  end.
+
