proof/LinearContext.v
@@ -1,0 +1,23 @@
+Set Warnings "-notation-overridden,-parsing".
+From PLF Require Import Maps.
+From Coq Require Import Lists.List.
+Import ListNotations.
+
+Definition linear_context (A : Type) := list (string * A).
+
+Definition empty {A:Type} : linear_context A := [].
+
+Definition find {A:Type} (ctx: linear_context A) (name: string) : option A.
+Admitted.
+
+Definition update {A : Type} (m : linear_context A) (x : string) (v : A) : linear_context A.
+Admitted.
+
+Definition rev_ctx {A : Type} (m : linear_context A): linear_context A.
+Admitted.
+
+Notation "x '|-c>' v ';' m" := (update m x v)
+                                (at level 100, v at next level, right associativity).
+Notation "x '|-c>' v" := (update empty x v)
+                          (at level 100).
+
