proof/Soundness.v
@@ -1,0 +1,35 @@
+Set Warnings "-notation-overridden,-parsing".
+From PLF Require Import Maps.
+From PLF Require Import Smallstep.
+From PLF Require Import CoreLang.
+From PLF Require Import LinearContext.
+From PLF Require Import NormalTypeSystem.
+From PLF Require Import RefinementType.
+From Coq Require Import Lists.List.
+Import ListNotations.
+
+(* Import RefinementType. *)
+
+Lemma has_refinement_type_has_basic_type: forall (e: tm) (tau: uty),
+    empty \C- e \T--> tau -> (Maps.empty |- e \in (erase tau)).
+Admitted.
+
+Global Hint Resolve has_refinement_type_has_basic_type: core.
+
+Theorem soundness: forall (e: tm) (T: basic_ty) (phi: constant -> Prop),
+    empty \C- e \T--> [[v: T | closed_r phi ]] ->
+    forall c, T = constant_basic_type_infer c -> phi c -> e -->* (tvalue (vconst c)).
+Proof with eauto.
+  intros e T phi H c HcT. subst.
+  assert (Maps.empty |- e \in (constant_basic_type_infer c )) as Hnt. apply has_refinement_type_has_basic_type in H...
+  induction H; intros.
+  - inversion Hnt; subst. destruct c; inversion H1. apply multi_R...
+  - admit.
+  - admit.
+  - admit.
+  - admit.
+  - admit.
+  - admit.
+  - admit.
+  - admit.
+Admitted.
